% Part: first-order-logic
% Chapter: syntax-and-semantics
% Section: discussion

\documentclass[../../../include/open-logic-section]{subfiles}

\begin{document}

\olfileid{fol}{dis}{quc}

\olsection{Interaction of quantifiers and connectives}

\paragraph{No operators} If $!C$ is a \emph{closed} formula:

\begin{itemize}
	\item $\forall x !C$ is equivalent to $!C$
	\item $\exists x !C$ is equivalent to $!C$
\end{itemize}

\paragraph{Negation} We have the following equivalences, called \emph{Duality}:

\begin{itemize}
	\item $\lnot \forall x !A$ is equivalent to $\exists x \lnot !A$.
	\item $\lnot \exists x !A$ is equivalent to $\forall x \lnot !A$.
\end{itemize}

Note that Duality implies the following:

\begin{itemize}
	\item $\lnot \forall x (!A \lif !B) $ is equivalent to $\exists x (!A \land \lnot !B)$.
	\item $\lnot \exists x (!A \land !B)$ is equivalent to $\forall x (!A \lif !\lnot !B)$.
\end{itemize}

Furthermore we have:

\begin{itemize}
	\item $\forall x \lnot !A \Entails \lnot \forall x !A$, but not the other way round unless $!A$ doesn't have free $x$.
	\item $\lnot \exists x !A \Entails \exists x \lnot !A$, but not the other way round unless $!A$ doesn't have free $x$.
\end{itemize}

\paragraph{Conjunction} We have:

\begin{itemize}
	\item $\forall x (!A \land !B)$ is equivalent to $\forall x !A \land \forall x !B$.
	\item $\exists x (!A \land !B) \Entails \exists x !A \land \exists x !B$, but not the other way round, though:
	\item if $!B$ doesn't have free $x$, $\exists x !A \land !B \Entails \exists x (!A \land !B)$ .
\end{itemize}

\paragraph{Disjunction} We have:

\begin{itemize}
	\item $\exists x (!A \lor !B)$ is equivalent to $\exists x !A \lor \exists x !B$.
	\item $\forall x !A \lor \forall x !B \Entails \forall x !A \lor \forall x !B$, but not the other way round, though:
	\item if $!B$ doesn't have free $x$, $\forall x !A \lor \forall x !B \Entails \forall x (!A \lor !B)$ .
\end{itemize}

\paragraph{Conditional} We have:

\begin{itemize}
	\item $\forall x (!A \lif !B) \Entails \forall x !A \lif \forall x !B$, but not the other way round,
	\item $\forall x (!A \lif !B) \Entails \exists x !A \lif \exists x !B$, but not the other way round,
	\item if $!A$ doesn't have free $x$, $!A \lif \forall x !B$ is equivalent to $\forall x (!A \lif !B)$.
\end{itemize}

\end{document}
