% Part: normal-modal-logic
% Chapter: axioms-systems
% Section: more-proofs-in-K

\documentclass[../../../include/open-logic-section]{subfiles}

\begin{document}

\olfileid{nml}{prf}{mpr}

\olsection{More Proofs in \Log{K}}

Let's see some more examples of !!{derivability} in~\Log{K}, now using
the simplified method introduced in \olref[der]{sec}.

\begin{prop}
  $\Log{K} \Proves \Box (!A \lif !B) \lif (\Diamond !A \lif \Diamond
  !B)$
\end{prop}

\begin{proof}
\begin{derivation}
1. & $\Log{K} \Proves (!A \lif !B) \lif (\lnot !B \lif \lnot !A)$ & \PL \\
2. &  $\Log{K} \Proves \Box(!A \lif !B) \lif (\Box\lnot!B \lif \Box\lnot!A)$ & \RK, 1 \\
3. & $\Log{K} \Proves (\Box\lnot!B \lif \Box\lnot!A) \lif (\lnot
\Box\lnot!A \lif \lnot\Box\lnot!B)$ & \Taut\\
4. & $\Log{K} \Proves \Box(!A \lif !B) \lif (\lnot
\Box\lnot!A \lif \lnot\Box\lnot!B)$ & \PL, 2, 3 \\
5. &  $\Log{K} \Proves \Box(!A \lif !B) \lif (\Diamond!A \lif \Diamond!B)$ & $\Diamond$ for $\lnot\Box\lnot$.
\end{derivation}
\end{proof}
  
\begin{prop}
$\Log{K}\Proves \Box!A \lif (\Diamond(!A \lif !B) \lif
  \Diamond !B)$
\end{prop}

\begin{proof}
  \begin{derivation}
  1. & $\Log{K} \Proves !A \lif (\lnot!B \lif \lnot (!A \lif !B))$ & \Taut \\
  2. & $\Log{K} \Proves \Box!A \lif  (\Box\lnot!B \lif \Box\lnot (!A\lif !B))$ &
  \RK, 1 \\
  3. &  $\Log{K} \Proves \Box!A \lif (\lnot \Box\lnot (!A\lif !B) \lif \lnot
  \Box\lnot!B)$ & \PL, 2 \\
  4. & $\Log{K} \Proves \Box!A \lif (\Diamond(!A \lif !B) \lif
  \Diamond !B)$ & $\Diamond$ for $\lnot\Box\lnot$.
  \end{derivation}
\end{proof}

\begin{prop}
  $\Log{K} \Proves (\Diamond!A \lor \Diamond!B) \lif \Diamond(!A \lor !B)$
\end{prop}

\begin{proof}
  \begin{derivation}
    1. & $\Log{K} \Proves \lnot(!A \lor !B) \lif \lnot!A$ & \Taut \\
    2. & $\Log{K} \Proves \Box\lnot(!A \lor !B) \lif \Box\lnot!A$ & \RK, 1 \\
    3. & $\Log{K} \Proves \lnot\Box\lnot !A \lif \lnot\Box\lnot(!A \lor!B)$ &
    \PL, 2\\
    4. & $\Log{K} \Proves \Diamond!A \lif \Diamond(!A \lor !B)$ &
    $\Diamond$ for $\lnot\Box\lnot$\\
    5. & $\Log{K} \Proves \Diamond!B \lif \Diamond(!A \lor !B)$ & similarly\\
    6. & $\Log{K} \Proves (\Diamond!A \lor\Diamond!B) \lif \Diamond(!A \lor !B)$
    & \PL, 4, 5.
  \end{derivation}
\end{proof}

\begin{prop}
  $\Log{K} \Proves \Diamond(!A \lor!B) \lif (\Diamond!A \lor \Diamond!B)$
\end{prop}

\begin{proof}
  \begin{derivation}
    1. & $\Log{K} \Proves \lnot !A \lif (\lnot !B \lif \lnot (!A \lor !B)$ & \Taut \\
    2. & $\Log{K} \Proves \Box\lnot !A \lif
    (\Box\lnot!B \lif \Box \lnot (!A \lor !B)$ & \RK\\
    3. & $\Log{K} \Proves \Box\lnot !A \lif (\lnot \Box \lnot (!A \lor!B)
    \lif \lnot\Box\lnot !B))$ & \PL, 2\\
    4. & $\Log{K} \Proves \lnot \Box \lnot(!A \lor !B) \lif (\Box \lnot !A \lif 
    \lnot\Box\lnot !B)$ & \PL, 3\\
    5. & $\Log{K} \Proves \lnot \Box \lnot(!A\lor!B) \lif (\lnot
    \lnot\Box\lnot!B \lif \lnot\Box\lnot!A)$ & \PL, 4\\
    6. & $\Log{K} \Proves \Diamond(!A \lor !B) \lif (\lnot
    \Diamond!B \lif \Diamond!A)$ & $\Diamond$ for $\lnot\Box\lnot$\\
    7. & $\Log{K} \Proves \Diamond(!A\lor!B) \lif (\Diamond!B \lor \Diamond!A)$ & \PL, 6. \\
  \end{derivation}
\end{proof}

\begin{prob}
  Show that the following !!{derivability} claims hold:
  \begin{enumerate}
  \item $\Log{K} \Proves \Diamond \lnot \lfalse \lif (\Box !A \lif
    \Diamond !A)$;
  \item $\Log{K} \Proves \Box(!A \lor !B) \lif (\Diamond !A \lor \Box
    !B)$;
  \item $\Log{K} \Proves (\Diamond !A \lif \Box !B) \lif \Box(!A \lif
    !B)$.
  \end{enumerate}
\end{prob}

\end{document}
