% Part: first-order-logic
% Chapter: axiomatic-deduction
% Section: provability-propositional

\documentclass[../../../include/open-logic-section]{subfiles}

\begin{document}

\iftag{FOL}
      {\olfileid{fol}{axd}{ppr}}
      {\olfileid{pl}{axd}{ppr}}

\olsection{\usetoken{S}{derivability} and the Propositional Connectives}

\begin{explain}
  We establish that the !!{derivability} relation~$\Proves$ of
  axiomatic deduction is strong enough to establish some basic facts
  involving the propositional connectives, such as that $!A \land !B
  \Proves !A$ and $!A, !A \lif !B \Proves !B$ (modus ponens). These
  facts are needed for the proof of the completeness theorem.
\end{explain}

\begin{prop}\ollabel{prop:provability-land}
  \begin{enumerate}
  \item \ollabel{prop:provability-land-left} Both $!A \land !B \Proves
    !A$ and $!A \land !B \Proves !B$
  \item \ollabel{prop:provability-land-right} $!A, !B \Proves !A \land !B$.
  \end{enumerate}
\end{prop}

\begin{proof}
  \begin{enumerate}
    \item From \olref[prp]{ax:land1} and \olref[prp]{ax:land1} by
      modus ponens.
  \item From \olref[prp]{ax:land3} by two applications of
    modus ponens.
  \end{enumerate}
\end{proof}


\begin{prop}\ollabel{prop:provability-lor}
  \begin{enumerate}
  \item $!A \lor !B, \lnot !A, \lnot !B$ is inconsistent.
  \item Both $!A \Proves !A \lor !B$ and $!B \Proves !A \lor !B$.
  \end{enumerate}
\end{prop}

\begin{proof}
  \begin{enumerate}
  \item From \olref[prp]{ax:lnot1} we get $\Proves \lnot !A \lif (!A
    \lif \lfalse)$ and $\Proves \lnot !B \lif (!B \lif \lfalse)$. So
    by the deduction theorem, we have $\{\lnot !A\} \Proves !A \lif
    \lfalse$ and $\{\lnot !B\} \Proves !B \lif \lfalse$. From
    \olref[prp]{ax:lor3} we get $\{\lnot !A, \lnot !B\} \Proves (!A
    \lor !B) \lif \lfalse$. By the deduction theorem, $\{!A \lor !B,
    \lnot !A, \lnot !B\} \Proves \lfalse$.
  \item From \olref[prp]{ax:lor1} and \olref[prp]{ax:lor2} by modus
    ponsens.
  \end{enumerate}
\end{proof}

\begin{prop}\ollabel{prop:provability-lif}
  \begin{enumerate}
  \item \ollabel{prop:provability-lif-left}  $!A, !A \lif !B \Proves !B$.
  \item \ollabel{prop:provability-lif-right}
    Both $\lnot !A \Proves !A \lif !B$ and $!B \Proves !A \lif !B$.
  \end{enumerate}
\end{prop}

\begin{proof}
  \begin{enumerate}
  \item We can !!{derive}:
    \begin{derivation}
      1. & $!A$ & \Hyp\\
      2. & $!A \lif !B$ & \Hyp\\
      3. & $!B$ & 1, 2, \MP
    \end{derivation}
    
  \item By \olref[prp]{ax:lnot2} and \olref[prp]{ax:lif1} and the
    deduction theorem, respectively.
  \end{enumerate}
\end{proof}

\end{document}
