\documentclass[../../../include/open-logic-section]{subfiles}

\begin{document}

\olfileid{sth}{replacement}{ref}
\olsection{Replacement and Reflection}

A final last attempt to justify Replacement, via \stagesinex, is to
consider a lovely result:
%In this, I will use overlining, such as $x_1, \ldots, x_n$, to
%abbreviate ``$x_1, \ldots, x_n$'': 
\begin{thm}[Reflection Schema]\ollabel{reflectionschema}
For any formula $\phi$:\footnote{But which may also have parameters}
\[
\forall \alpha \exists \beta > \alpha (\forall x_1 \ldots, x_n \in
V_\beta)(\phi(x_1, \ldots, x_n) \liff \phi^{V_\beta}(x_1, \ldots, x_n))
\]
\end{thm}

As before, $\phi^{V_\beta}$ is the result of restricting every
quantifier in $\phi$ to the set $V_\beta$. So, intuitively, Reflection
says this: if $\phi$ is true in the entire hierarchy, then $\phi$ is
true in arbitrarily many \emph{initial segments} of the hierarchy. 

\citet{Montague1961} and \citet{Levy1960} showed that (suitable
formulations of) Replacement and Reflection are equivalent,
modulo~$\Z$, so that adding either gives you~$\ZF$. So, given this
equivalence, one might hope to justify Reflection  and Replacement via
\stagesinex{} as follows: given \stagesinex, the hierarchy should be
very, very tall; so tall, in fact, that nothing we can say about it is
sufficient to bound its height. And we can understand this as the
thought that, if any sentence~$\phi$ is true in the entire hierarchy,
then it is true in arbitrarily many initial segments of the hierarchy.
And that is just Reflection. 

Again, this seems like a genuinely promising attempt to provide an
intrinsic justification for Replacement. But there is much too much to
say about it here. You must now decide for yourself whether it
succeeds.

Finally, we will prove that Replacement entails
Reflection. This is easily the most advanced bit of mathematics in
this textbook (so if you follow it, well done). We'll start with a
lemma which, for brevity, employs the notational device of
\emph{overlining} to deal with sequences of variables or objects. So:
``$\overline{a}_k$'' abbreviates ``$a_{k_1}$, \dots, $a_{k_n}$'', where
$n$ is determined by context.

\begin{lem}\ollabel{lemreflection}
For each $1 \leq i \leq k$, let $\phi_i(\overline{v}_i, x)$ be a
formula.\footnote{Which may have parameters.} Then for each $\alpha$
there is some $\beta > \alpha$ such that, for any $\overline{a}_1,
\ldots, \overline{a}_k \in V_\beta$ and each $1 \leq i \leq k$:
\[
	\exists x\phi_i(\overline{a}_i, x) \rightarrow (\exists x \in V_\beta) \phi_i(\overline{a}_i, x)
\]
\end{lem}

\begin{proof}
We define a term $\mu$ as follows: $\mu(\overline{a}_1, \ldots,
\overline{a}_k)$ is the least stage, $V$, which satisfies all of the
following conditionals, for $1 \leq i \leq k$:
\[
\exists x\phi_i(\overline{a}_i, x) \rightarrow (\exists x \in V) \phi_i(\overline{a}_i, x))
\]
Using Replacement and our recursion theorem, define:
\begin{align*}
	S_0 & = V_{\alpha+1}\\
	S_{m+1} & = S_m \cup \bigcup
	\Setabs{\mu(\overline{a}_1, \ldots, \overline{a}_k)}
	{\overline{a}_1, \ldots, \overline{a}_k \in S_m} \\
	S &= \bigcup_{m < \omega} S_m.
\end{align*}
Each $S_m$, and hence $S$ itself, is a stage after $V_\alpha$. Now fix
$\overline{a}_1$, \dots,~$\overline{a}_k \in S$; so there is some $m <
\omega$ such that $\overline{a}_1$, \dots, $\overline{a}_k \in S_m$.
Fix some $1 \leq i \leq k$, and suppose that $\exists x
\phi_i(\overline{a}_i,x)$. So $(\exists x \in \mu(\overline{a}_1,
\ldots, \overline{a}_k))\phi_i(\overline{a}_i, x)$ by construction, so
$(\exists x \in S_{m+1})\phi_i(\overline{a}_i, x)$ and hence
$(\exists x \in S)\phi_i(\overline{a}_i, x)$. So $S$ is our $V_\beta$.
\end{proof}

From here, we can prove \olref{reflectionschema} quite
straightforwardly:

\begin{proof}[Proof of \olref{reflectionschema}] 
Fix $\alpha$. Without loss of generality, we can assume $\phi$'s only
connectives are $\exists$, $\lnot$ and $\land$ (since these are
expressively adequate). Let $\psi_1, \ldots, \psi_k$ enumerate each of
$\phi$'s subformulas according to complexity, so that $\psi_k = \phi$.
By \olref{lemreflection}, there is a $\beta > \alpha$ such that, for
any $\overline{a}_i \in V_\beta$ and each $1 \leq i \leq k$:
\begin{align}\label{reflectionnicelybehaved}
	\exists x\psi_i(\overline{a}_i, x) \rightarrow 
	(\exists x \in V_\beta) \psi_i(\overline{a}_i, x)\tag{*}
\end{align}
By induction on complexity of $\psi_i$, we will show that
$\psi_i(\overline{a}_i) \leftrightarrow
\psi_i^{V_\beta}(\overline{a}_i)$, for any  $\overline{a}_i \in
V_\beta$. 	If $\psi_i$ is atomic, this is trivial. The biconditional
also establishes that, when $\psi_i$ is a negation or conjunction of
subformulas satisfying this property, $\psi_i$ itself satisfies this
property. So the only interesting case concerns quantification. Fix
$\overline{a}_i \in V_\beta$; then:
\begin{align*}
	(\exists x \psi_i(\overline{a}_i, x))^{V_\beta}
	&\text{ iff }
	(\exists x \in V_\beta)\psi_i^{V_\beta}(\overline{a}_i, x)
	&&\text{by definition}\\
	&\text{ iff }
	(\exists x \in V_\beta)\psi_i(\overline{a}_i,  x)
	&&\text{by the induction hypothesis}\\
	&\text{ iff }
	\exists x \psi_i(\overline{a}_i, x)
	&&\text{by \eqref{reflectionnicelybehaved}}
\end{align*}
This completes the induction; the result follows as $\psi_k = \phi$.
\end{proof}

We have shown in $\ZF$ that Reflection holds. The proof essentially
followed \citet{Montague1961}. We now want to prove in $\Z$ that
Reflection entails Replacement. The proof follows \citet{Levy1960},
but with a simplification. 

Since we are working in $\Z$, we cannot present Reflection in exactly
the form given above. After all, we formulated Reflection using the
``$V_\alpha$'' notation, and that cannot be defined in $\Z$. So
instead we will offer an apparently weaker formulation of Replacement,
as follows:

\ \\\emph{Weak-Reflection.} For any formula $\phi$, there is a
transitive set $S$ such that $0$, $1$, and any parameters to $\phi$
are !!{element}s of $S$, and $(\forall \overline{x} \in S)(\phi \liff
\phi^S)$.

\
\\
To use this to prove Replacement, we will first follow \citet[first
part of Theorem 2]{Levy1960} and show that we can ``reflect'' two
formulas at once:

\begin{lem}[in $\Z + \text{Weak-Reflection}$.]\ollabel{lem:reflect}
For any formulas $\psi, \chi$, there is a transitive set $S$ such that $0$ and $1$ (and any parameters to the formulas) are !!{element}s of $S$, and $(\forall \overline{x} \in S)((\psi \liff \psi^S) \land (\chi \liff \chi^S))$.
\end{lem}

\begin{proof}
Let $\phi$ be the formula $(z = 0 \land \psi) \lor (z = 1 \land \chi)$. 

Here we use an abbreviation; we should spell out ``$z = 0$'' as
``$\forall t\, t \notin z$'' and ``$z =1$'' as ``$\forall s(s \in z
\liff \forall t\, t \notin s)$''. But since $0, 1 \in S$ and $S$ is
transitive, these formulas are \emph{absolute} for $S$; that is, they
will apply to the same object whether we restrict their quantifiers to
$S$.\footnote{More formally, letting $\xi$ be either of these
formulas, $\xi(z) \liff \xi^S(z)$.}

By Weak-Reflection, we have some appropriate $S$ such that:
\begin{align*}
	(\forall z, \overline{x} \in S)(&\phi \liff \phi^S)\\
	(\forall z, \overline{x} \in S)(&((z = 0 \land \psi) \lor (z = 1 \land \chi)) \liff 
	((z = 0 \land \psi) \lor (z = 1 \land \chi))^S)\\
	(\forall z, \overline{x} \in S)(&((z = 0 \land \psi) \lor (z = 1 \land \chi))\liff ((z = 0 \land \psi^S) \lor (z = 1 \land \chi^S)))\\
	(\forall \overline{x} \in S)(&(\psi \liff \psi^S) \land (\chi \liff \chi^S))
\end{align*}
The second claim entails the third because ``$z = 0$'' and ``$z=1$''
are absolute for $S$; the fourth claim follows since $0 \neq 1$.
\end{proof}\noindent We now obtain Replacement, simplifying
\citet[Theorem 6]{Levy1960}:

\begin{thm}[in $\Z$ + Weak-Reflection]\label{thm:replacement} 
For any formula $\phi(v,w)$,\footnote{Which may contain parameters}
and any $A$, if $(\forall x \in A)\lexists![y][\phi(x,y)]$, then
$\Setabs{y}{(\exists x \in A)\phi(x,y}$ exists.
\end{thm}

\begin{proof}
Fix $A$ such that $(\forall x \in A)\lexists![y][\phi(x,y)]$, and
define some formulas:
\begin{align*}
	\psi &\text{ is } (\phi(x, z) \land A = A)\\
	\chi &\text{ is } \lexists[y][\phi(x, y)]
\end{align*}
Using \olref{lem:reflect}, since $A$ is a parameter to $\psi$, there
is a transitive~$S$ such that $0, 1, A \in S$  (along with any other
parameters), and such that:
\[
	(\forall x,z \in S)((\psi \liff \psi^S) \land (\chi \liff \chi^S))
\]
So in particular:
\begin{align*}
	(\forall  x, z \in S)(&\phi(x, z) \liff \phi^S(x, z))\\
	(\forall x \in S)(&\exists y\phi(x, y) \liff (\exists y \in S)\phi^S(x, y)) 
\end{align*}
Combining these, and observing that $A \subseteq S$ since $A \in S$ and $S$ is transitive:
\begin{align*}
	(\forall x \in A)(&\exists y\phi(x, y) \liff (\exists y \in S)\phi(x, y))
\end{align*}
Now $(\forall x \in A)(\lexists![y \in S])\phi(x, y)$, because
$(\forall x \in A)\lexists![y][\phi(x, y)]$. Now Separation yields
$\Setabs{y \in S}{(\exists x \in A) \phi(x, y)} = \Setabs{y}{(\exists
x \in A) \phi(x, y)}$. 
\end{proof}

%\begin{thm}[\emph{working in $\Z$}] If every instance of this scheme holds:
%	\begin{enumerate}
%		\item[] \emph{Reflection$^*$.} For any formula $\phi$ with parameters $A_1, \ldots, A_n$, there is some set $S$ which both has all parameters as members and subsets, and such that $\phi \liff \phi^S$.
%	\end{enumerate}
%	then every instance of the Replacement Schema holds.
%\end{thm}

\end{document}